Weidenbach_Book/Propo_CDCL_Termination.thy
@@ -5,7 +5,7 @@ begin
 text \<open>The condition that no learned clause is a tautology is overkill (in the sense that the
   no-duplicate condition is enough), but we can reuse @{term build_all_simple_clss}.\<close>
 definition cdcl_all_inv_mes where
-  "cdcl_all_inv_mes S =
+  "cdcl_all_inv_mes S =     
     (no_strange_atm S \<and> cdcl_M_level_inv S \<and>  finite (atms_of_m (clauses S))
     \<and>  finite (learned_clauses S) \<and>  (\<forall>s \<in> learned_clauses S. \<not>tautology s)
     \<and>  distinct_cdcl_state S \<and> cdcl_conflicting S
